src/lib/poly/gemm/Kuiper.Poly.GEMM.OrigBlockTiling1D.fsti
@@ -3,11 +3,48 @@ module Kuiper.Poly.GEMM.OrigBlockTiling1D
 #lang-pulse
 
 open Kuiper
+open Kuiper.Approximates
 open Kuiper.Poly.GEMMGPU.Type
 open Kuiper.Matrix
 open Kuiper.EMatrix
 open Kuiper.Matrix.Reprs.Type
 module MS = Kuiper.Spec.GEMM
+module MU = Kuiper.Poly.GEMM.Util
+
+inline_for_extraction noextract
+fn mmcomb_gpu_approx
+  (#et : Type0) {| scalar et, real_like et |}
+  (comb : binop et)
+  (comb_r : binop real { forall x y r s. x %~ r /\ y %~ s ==> comb x y %~ comb_r r s })
+  (bm bn bk : szp)
+  (#mrows #mshared #mcols : szp)
+  (tm : szp{tm /?+ bm})
+  (#_: squash ((bm/tm * bn) == bm * bk /\ (bm/tm * bn) == bn * bk))
+  (#lA : mlayout (mrows   * bm) (mshared * bk))
+  (#lB : mlayout (mshared * bk) (mcols   * bn))
+  (#lC : mlayout (mrows   * bm) (mcols   * bn))
+  {| clayout lA, clayout lB, clayout lC |}
+  (gA : gpu_matrix et lA { is_global_matrix gA })
+  (#fA : perm)
+  (gB : gpu_matrix et lB { is_global_matrix gB })
+  (#fB : perm)
+  (gC : gpu_matrix et lC { is_global_matrix gC })
+  (#eA : ematrix et (mrows   * bm) (mshared * bk))
+  (#eB : ematrix et (mshared * bk) (mcols   * bn))
+  (#eC : ematrix et (mrows   * bm) (mcols   * bn))
+  norewrite
+  preserves
+    cpu **
+    on gpu_loc (gA |-> Frac fA eA) **
+    on gpu_loc (gB |-> Frac fB eB)
+  requires
+    pure (mrows * mcols <= max_blocks) **
+    pure (bm/tm * bn <= max_threads) **
+    on gpu_loc (gC |-> eC)
+  ensures
+    (exists* (eC' : ematrix et _ _).
+      on gpu_loc (gC |-> eC') **
+      pure (ematrix_approximates eC' (MU.real_mmcomb comb_r eC eA eB)))
 
 inline_for_extraction noextract
 fn mmcomb_gpu
